Update delta- and gamma-rules to make them more robust by explicitely selecting the relevant variable/symbol (#13)
Closes: #3.

Update the rules in `ATPCompat` so that, instead of having a brittle
`add y S` in conclusion of `hasTableauAll` (which can easily break
depending on the order of the metavariable set passed at the start of
the proof), we postulate that there is an `S0` such that `S0 = rem y S`
and `set_in y S`. This allows to derive that `S = add y S0`. We do the
same thing for Skolemization rules with the skolem symbol.

theories/Prelude/Sets.v
@@ -22,6 +22,7 @@ Class set {A : Type} :=
   ; set_in : A -> car -> Prop    (** Use [mem_spec] to convert [mem] to [set_in] in proofs *)
   ; union : car -> car -> car
   ; inter : car -> car -> car
+  ; diff  : car -> car -> car
   ; singleton : A -> car
 
   (** *** Extensionality property of sets *)
@@ -32,7 +33,9 @@ Class set {A : Type} :=
   ; mem_spec : forall (x : A) (s : car), mem x s = true <-> set_in x s
   ; singleton_spec : forall (x y : A), set_in x (singleton y) <-> x = y
   ; union_spec : forall (x : A) (s1 s2 : car), set_in x (union s1 s2) <-> set_in x s1 \/ set_in x s2
-  ; inter_spec : forall (x : A) (s1 s2 : car), set_in x (inter s1 s2) <-> set_in x s1 /\ set_in x s2 }.
+  ; inter_spec : forall (x : A) (s1 s2 : car), set_in x (inter s1 s2) <-> set_in x s1 /\ set_in x s2
+  ; diff_spec  : forall (x : A) (s1 s2 : car), set_in x (diff s1 s2) <-> set_in x s1 /\ ~ set_in x s2
+  }.
 Arguments set : clear implicits.
 
 Notation "S1 \union S2" := (union S1 S2) (at level 30).
@@ -40,6 +43,18 @@ Notation "S1 \inter S2" := (inter S1 S2) (at level 25).
 
 Section SetProperties.
   Context {A : Type} `{set_A : set A}.
+
+  Lemma carrier_eq_dec :
+    forall (x y : A), x = y \/ x <> y.
+  Proof using set_A.
+    intros. destruct (singleton x == singleton y) as [e | n].
+    - rewrite set_ext in e. specialize (e x).
+      destruct e as (h & _).
+      have hin : set_in x (singleton x) by now rewrite singleton_spec.
+      specialize (h hin). rewrite singleton_spec in h. now left.
+    - rewrite set_ext in n. right. intro e.
+      apply n. intro z. subst. tauto.
+  Qed.
 
   Definition add (x : A) (s : set_A) : set_A :=
     union (singleton x) s.
@@ -75,6 +90,48 @@ Section SetProperties.
     - apply add_inv in hin. destruct hin.
       + rewrite H. now apply singleton_spec.
       + now apply empty_spec in H.
+  Qed.
+
+  Definition rem (x : A) (s : set_A) : set_A :=
+    diff s (singleton x).
+
+  Lemma rem_spec1 :
+    forall (x : A) (s : set_A),
+      ~ set_in x (rem x s).
+  Proof using Type.
+    intros ?? hin; unfold rem in hin.
+    rewrite diff_spec in hin. destruct hin as (_ & h). apply h.
+    now apply singleton_spec.
+  Qed.
+
+  Lemma rem_spec2 :
+    forall (x y : A) (s : set_A),
+      set_in y (rem x s) -> set_in y s.
+  Proof using Type.
+    intros ??? h. unfold rem in h.
+    rewrite diff_spec in h. now destruct h as [hin _].
+  Qed.
+
+  Lemma rem_spec3 :
+    forall (x y : A) (s : set_A),
+      x <> y -> set_in y s -> set_in y (rem x s).
+  Proof using Type.
+    intros ??? n e. unfold rem. rewrite diff_spec.
+    split; auto. intro contra. apply n.
+    now rewrite singleton_spec in contra.
+  Qed.
+
+  Lemma add_rem :
+    forall (x : A) (s : set_A),
+      set_in x s -> add x (rem x s) = s.
+  Proof using Type.
+    intros. apply set_ext; intro y; split; intro h.
+    - apply add_inv in h. destruct h as [e | h]; subst; auto.
+      eapply rem_spec2; eauto.
+    - unfold add. rewrite union_spec.
+      destruct (carrier_eq_dec x y) as [e | n].
+      + left. rewrite e. now rewrite singleton_spec.
+      + right. eapply rem_spec3; eauto.
   Qed.
 
   Definition subset (s1 s2 : set_A) :=
@@ -340,6 +397,18 @@ Module SetComputationalInstances.
       intros; rewrite SetOfX_.singleton_spec. reflexivity.
     Qed.
 
+    Lemma SetOfX_diff_spec :
+      forall (x : X.t) (s1 s2 : SetOfX_.t),
+        SetOfX_.In x (SetOfX_.diff s1 s2) <-> SetOfX_.In x s1 /\ ~ SetOfX_.In x s2.
+    Proof.
+      intros; split; intro H.
+      - split.
+        + eapply SetOfXFacts.diff_1; eauto.
+        + intro contra. now apply SetOfXFacts.diff_2 in H.
+      - destruct H as (hin & hnin).
+        apply SetOfXFacts.diff_3; auto.
+    Qed.
+
     Lemma SetOfX_equal_eq :
       forall x y : SetOfX_.t, SetOfX_.equal x y = true <-> x = y.
     Proof.
@@ -365,6 +434,7 @@ Module SetComputationalInstances.
       ;  set_in := SetOfX_.In
       ;  union := SetOfX_.union
       ;  inter := SetOfX_.inter
+      ;  diff := SetOfX_.diff
       ;  singleton := SetOfX_.singleton
 
       ;  set_ext := SetOfX_set_ext
@@ -373,7 +443,8 @@ Module SetComputationalInstances.
       ;  singleton_spec := SetOfX_singleton_spec
       ;  mem_spec x s := SetOfX_.mem_spec s x
       ;  union_spec x s1 s2 := SetOfX_.union_spec s1 s2 x
-      ;  inter_spec x s1 s2 := SetOfX_.inter_spec s1 s2 x |}.
+      ;  inter_spec x s1 s2 := SetOfX_.inter_spec s1 s2 x
+      ;  diff_spec := SetOfX_diff_spec |}.
   End SetFromOrdered.
 
   (** Set of natural numbers. *)
