devtools/tests/instantiate_apply.v
@@ -13,13 +13,18 @@ Theorem T_proof:
 Proof.
   exists\{ "Y5_12"\}, \{ "skolem@X7@0"\}.
   unshelve eapply hasTableauNegAll with (sko := OuterSkolemization) (i := 0).
-  1, 2: shelve.
+  1-3: shelve.
   1: exact((EFun "skolem@X7@0"[])).
   2, 3: reflexivity.
   1: { now esimpl. }
+  1: { now esimpl. }
   eapply hasTableauNegImp with (i := 0).
   1: { reflexivity. }
-  eapply hasTableauNegEx with(i := 1).
+  unshelve eapply hasTableauNegEx with(i := 1).
+  1-3: shelve.
+  1: exact "Y5_12".
+  1: { reflexivity. }
+  1: { now esimpl. }
   1: { reflexivity. }
   1: { now esimpl. }
   eapply hasTableauNegOr with(i := 0).
